src/test.lean
@@ -1,4 +1,5 @@
 import tactic.ext
+import data.set.basic
 
 section
 variable (α : Type)
@@ -8,3 +9,5 @@ structure TestStruct :=
 (x : α)
 
 end
+
+#check set.preimage_image_eq
