src/verification/ident.lean
@@ -1,0 +1,58 @@
+import tactic.derive_fintype
+
+section Ident
+
+section vars
+@[derive decidable_eq, derive fintype, derive inhabited]
+inductive Vars
+| i | j | k | w | x | y | z | ind₀ | ind₁ | ind₂ | break | output
+
+open Vars
+instance : has_to_string Vars :=
+⟨λ v, match v with 
+-- S.split(" | ").map(s => s + ' := "' + s + '"')
+| i := "i" | j := "j" | k := "k" | w := "w" | x := "x" | y := "y" | z := "z" | ind₀ := "ind₀" | ind₁ := "ind₁" | ind₂ := "ind₂" | break := "break" | output := "output"
+end⟩
+end vars
+
+section NameSpace
+@[derive decidable_eq, derive inhabited, derive has_to_string, reducible]
+def NameSpace := ℕ
+
+def NameSpace.reserved : NameSpace := 0
+
+def fresh (S : finset NameSpace) : NameSpace :=
+S.max.iget + 1
+
+theorem not_fresh_mem (S : finset NameSpace) : fresh S ∉ S :=
+begin
+  simp only [fresh],
+  cases hn : S.max,
+  { rw [finset.max_eq_none] at hn, subst hn, exact finset.not_mem_empty _, },
+  intro h, simpa using finset.le_max_of_mem h hn,
+end
+
+theorem not_fresh_reserved (S : finset NameSpace) : fresh S ≠ NameSpace.reserved :=
+by simp [fresh, NameSpace.reserved]
+
+attribute [irreducible] NameSpace
+end NameSpace
+
+@[derive decidable_eq]
+structure Ident :=
+(ns : NameSpace)
+(name : Vars)
+
+@[simp] lemma Ident_ns (ns : NameSpace) (name : Vars) :
+  (Ident.mk ns name).ns = ns := rfl
+
+@[simp] lemma Ident_name (ns : NameSpace) (name : Vars) :
+  (Ident.mk ns name).name = name := rfl
+-- def Ident.of : string → Ident := Ident.name
+instance : has_to_string Ident :=
+⟨λ i, "n" ++ (to_string i.ns) ++ "_" ++ (to_string i.name)⟩
+
+@[simp] lemma Ident_ns_range : set.range Ident.ns = set.univ :=
+by { ext, simp, exact ⟨⟨x, default⟩, rfl⟩, }
+
+end Ident
